WIP: basic_step refactoring + fixing some admits

Coq/src/Step.v
@@ -2,7 +2,7 @@ Require Import Omega.
 From hahn Require Import Hahn.
 From promising Require Import Basic.
 From imm Require Import Events AuxRel. 
-Require Import AuxRel AuxDef EventStructure Consistency.
+Require Import AuxRel AuxDef EventStructure Consistency BasicStep.
 
 Set Implicit Arguments.
 
@@ -56,3 +56,664 @@ Notation "'K' S" := (S.(ES.cont_set)) (at level 10).
 
 Notation "'Tid' S" := (fun t e => S.(ES.tid) e = t) (at level 9).
 
+Definition add_jf (r : eventid) (S S' : ES.t) : Prop :=
+  ⟪ RR : R S' r ⟫ /\
+  exists w,
+    ⟪ EW  : S.(ES.acts_set) w ⟫ /\
+    ⟪ WW  : W S' w ⟫ /\
+    ⟪ LOC : same_loc S' w r ⟫ /\
+    ⟪ VAL : same_val S' w r ⟫ /\
+    ⟪ JF' : S'.(ES.jf) ≡ S.(ES.jf) ∪ singl_rel w r ⟫.
+
+Definition add_ew (w : eventid) (S S' : ES.t) : Prop :=
+  ⟪ WW : W S' w ⟫ /\
+  exists (ws : eventid -> Prop),
+    ⟪ WWS   : ws ⊆₁ W S ⟫ /\
+    ⟪ LOCWS : ws ⊆₁ same_loc S w ⟫ /\
+    ⟪ VALWS : ws ⊆₁ same_val S w ⟫ /\
+    ⟪ CFWS  : ws ⊆₁ S.(ES.cf) w ⟫ /\
+    ⟪ REPR :
+      S'.(ES.ew) ≡ S.(ES.ew) ∪ ws × eq w ∪ eq w × ws ⟫.
+
+Definition add_co (w : eventid) (S S' : ES.t) : Prop :=
+  let A := S.(ES.acts_set) ∩₁ W S ∩₁ (same_loc S w) \₁ (S.(ES.cf)^? w) in
+  ⟪ WW : W S' w ⟫ /\
+  exists (ws : eventid -> Prop),
+    ⟪ WWS : ws ⊆₁ A ⟫ /\
+    ⟪ REPR :
+      S'.(ES.co) ≡ S.(ES.co) ∪ S.(ES.ew) ∪ ws × eq w ∪ eq w × (A \₁ ws) ⟫.
+
+Definition t_fence
+           (e  : eventid)
+           (e' : option eventid)
+           (S S' : ES.t) : Prop :=
+  ⟪ ENONE : e' = None ⟫ /\
+  ⟪ FF  : F S' e ⟫ /\
+  ⟪ JF' : S'.(ES.jf) ≡ S.(ES.jf) ⟫ /\
+  ⟪ EW' : S'.(ES.ew) ≡ S.(ES.ew) ⟫ /\
+  ⟪ CO' : S'.(ES.co) ≡ S.(ES.co) ⟫.
+
+Definition t_load
+           (e  : eventid)
+           (e' : option eventid)
+           (S S' : ES.t) : Prop :=
+  ⟪ ENONE : e' = None ⟫ /\
+  ⟪ AJF : add_jf e S S' ⟫ /\
+  ⟪ EW' : S'.(ES.ew) ≡ S.(ES.ew) ⟫ /\
+  ⟪ CO' : S'.(ES.co) ≡ S.(ES.co) ⟫.
+
+Definition t_store
+           (e  : eventid)
+           (e' : option eventid)
+           (S S' : ES.t) : Prop :=
+  ⟪ ENONE : e' = None ⟫ /\
+  ⟪ JF' : S'.(ES.jf) ≡ S.(ES.jf) ⟫ /\
+  ⟪ AEW : add_ew e S S' ⟫ /\
+  ⟪ ACO : add_co e S S' ⟫.
+
+Definition t_update
+           (e  : eventid)
+           (e' : option eventid)
+           (S S' : ES.t) : Prop := exists w,
+  ⟪ ESOME : e' = Some w ⟫ /\
+  ⟪ AJF : add_jf e S S' ⟫ /\
+  ⟪ AEW : add_ew w S S' ⟫ /\
+  ⟪ ACO : add_co w S S' ⟫.
+
+Definition t_ e e' S S' :=
+  t_fence e e' S S' \/ t_load e e' S S' \/ t_store e e' S S' \/ t_update e e' S S'.
+
+Definition t (m : model) (S S' : ES.t) : Prop := exists e e',
+  ⟪ TT  : t_ e e' S S' ⟫ /\
+  ⟪ BSTEP : ESBasicStep.t e e' S S' ⟫ /\
+  ⟪ CON : @es_consistent S' m ⟫.
+
+(******************************************************************************)
+(** ** Load step properties *)
+(******************************************************************************)
+
+Lemma load_step_E e e' S S'
+      (BSTEP : ESBasicStep.t e e' S S')
+      (LSTEP: t_load e e' S S') :
+  E S' ≡₁ E S ∪₁ eq e.
+Proof. 
+  assert (e' = None) by inv LSTEP. subst.
+    by apply ESBasicStep.basic_step_nupd_acts_set.
+Qed.
+
+Lemma load_step_R e e' S S'
+      (LSTEP: t_load e e' S S') :
+  R S' e.
+Proof. apply LSTEP. Qed.
+
+Lemma load_step_r e e' S S'
+      (BSTEP : ESBasicStep.t e e' S S')
+      (LSTEP: t_load e e' S S') 
+      (wfE: ES.Wf S) :
+  E S' ∩₁ R S' ≡₁ (E S ∩₁ R S) ∪₁ eq e.
+Proof. 
+  erewrite load_step_E; eauto.
+  rewrite set_inter_union_l.
+  arewrite (eq e ∩₁ R S' ≡₁ eq e).
+  { generalize (load_step_R LSTEP).
+    basic_solver. }
+  arewrite (E S ∩₁ R S' ≡₁ E S ∩₁ R S). 2: done.
+  eapply ESBasicStep.type_step_eq_dom; eauto.
+Qed.  
+
+Lemma load_step_w e e' S S'
+      (BSTEP : ESBasicStep.t e e' S S')
+      (LSTEP: t_load e e' S S') 
+      (wfE: ES.Wf S) :
+  E S' ∩₁ W S' ≡₁ E S ∩₁ W S.
+Proof. 
+  assert (R S' e) as AA.
+  { eapply load_step_R; eauto. }
+  erewrite load_step_E; eauto.
+  rewrite set_inter_union_l.
+  arewrite (E S ∩₁ W S' ≡₁ E S ∩₁ W S).
+  { eapply ESBasicStep.type_step_eq_dom; eauto. }
+  arewrite (eq e ∩₁ W S' ≡₁ ∅).
+  { split; [|basic_solver].
+    unfolder. ins. desf.
+    type_solver. }
+  basic_solver.
+Qed.  
+
+Lemma load_step_f e e' S S'
+      (BSTEP : ESBasicStep.t e e' S S')
+      (LSTEP: t_load e e' S S') 
+      (wfE: ES.Wf S) :
+  E S' ∩₁ F S' ≡₁ E S ∩₁ F S.
+Proof. 
+  assert (R S' e) as AA.
+  { eapply load_step_R; eauto. }
+  erewrite load_step_E; eauto.
+  rewrite set_inter_union_l.
+  arewrite (E S ∩₁ F S' ≡₁ E S ∩₁ F S).
+  { eapply ESBasicStep.type_step_eq_dom; eauto. }
+  arewrite (eq e ∩₁ F S' ≡₁ ∅).
+  { split; [|basic_solver].
+    unfolder. ins. desf.
+    type_solver. }
+  basic_solver.
+Qed.
+
+Lemma load_step_rel e e' S S'
+      (BSTEP : ESBasicStep.t e e' S S')
+      (LSTEP: t_load e e' S S') 
+      (wfE: ES.Wf S) :
+  E S' ∩₁ FW S' ∩₁ Rel S' ≡₁ E S ∩₁ FW S ∩₁ Rel S.
+Proof. 
+  cdes LSTEP; cdes AJF; cdes BSTEP; cdes BSTEP_.
+  rewrite set_inter_union_r, load_step_w, load_step_f; eauto.
+  rewrite <- set_inter_union_r.
+  rewrite (set_interC (E S)).
+  rewrite set_interA.
+  arewrite (E S ∩₁ Rel S' ≡₁ E S ∩₁ Rel S); [|basic_solver].
+  unfold is_rel, mode_le. 
+  unfolder. splits; intros x [xE HH].
+  { erewrite ESBasicStep.basic_step_mod_eq_dom in HH; eauto. }
+  erewrite <- ESBasicStep.basic_step_mod_eq_dom in HH; eauto. 
+Qed.
+
+Lemma load_step_acq e e' S S'
+      (BSTEP : ESBasicStep.t e e' S S')
+      (LSTEP: t_load e e' S S') 
+      (wfE: ES.Wf S) :
+  E S' ∩₁ FR S' ∩₁ Acq S' ≡₁ (E S ∩₁ FR S ∩₁ Acq S) ∪₁ (eq e ∩₁ Acq S').
+Proof. 
+  cdes LSTEP; cdes AJF; cdes BSTEP; cdes BSTEP_.
+  rewrite set_inter_union_r, load_step_r, load_step_f; eauto.
+  rewrite <- set_unionA.
+  rewrite <- set_inter_union_r.
+  rewrite set_inter_union_l.
+  arewrite (E S ∩₁ FR S ∩₁ Acq S' ≡₁ E S ∩₁ FR S ∩₁ Acq S); auto.
+  unfold is_acq, mode_le. 
+  unfolder; splits; intros x [[xE xFR] HH].
+  { erewrite ESBasicStep.basic_step_mod_eq_dom in HH; eauto. }
+  erewrite <- ESBasicStep.basic_step_mod_eq_dom in HH; eauto.
+Qed.  
+
+Lemma load_step_jf_dom e e' S S'
+      (BSTEP : ESBasicStep.t e e' S S')
+      (LSTEP: t_load e e' S S') 
+      (wfE: ES.Wf S) : 
+  dom_rel (jf S') ⊆₁ E S.
+Proof. 
+  cdes LSTEP; cdes AJF; cdes BSTEP; cdes BSTEP_.
+  rewrite JF', dom_union. 
+  apply set_subset_union_l.
+  rewrite wfE.(ES.jfE).
+  basic_solver.
+Qed.
+
+Lemma load_step_jfe_dom e e' S S'
+      (BSTEP : ESBasicStep.t e e' S S')
+      (LSTEP: t_load e e' S S') 
+      (wfE: ES.Wf S) : 
+  dom_rel (jfe S') ⊆₁ E S.
+Proof. 
+  unfold ES.jfe.
+  unfolder; ins; desf.
+  eapply load_step_jf_dom; eauto. 
+  basic_solver.
+Qed.  
+
+Lemma load_step_jfe e e' S S'
+      (BSTEP : ESBasicStep.t e e' S S')
+      (LSTEP: t_load e e' S S') 
+      (wfE: ES.Wf S) : 
+  jfe S' ≡ jfe S ∪ jfe S' ⨾ ⦗eq e⦘.
+Proof. 
+  cdes LSTEP; cdes AJF; cdes BSTEP; cdes BSTEP_.
+  unfold ES.jfe.
+  erewrite ESBasicStep.basic_step_nupd_sb. 
+  2 : { desf; eauto. }
+  rewrite <- EVENT.
+  rewrite JF'.
+  rewrite minus_union_l at 1.
+  apply union_more.
+  { rewrite ES.sbE, ES.jfE; auto. 
+    rewrite minus_union_r. 
+    erewrite minus_disjoint with (r' := ES.cont_sb_dom S k × eq e). 
+    2 : { unfolder; splits; ins; desf; omega. }
+    basic_solver. }
+  rewrite <- seq_eqv_minus_lr, seq_union_l. 
+  arewrite (jf S ⨾ ⦗eq e⦘ ≡ ∅₂). 
+  { rewrite wfE.(ES.jfE).
+    unfolder; splits; ins; desf; omega. }
+  basic_solver 10.
+Qed.
+
+Lemma load_step_sb_jf  lang k k' st st' e e' S S'
+      (BSTEP_ : ESBasicStep.t_ lang k k' st st' e e' S S') 
+      (LSTEP: t_load e e' S S') 
+      (wfE: ES.Wf S) :
+  (sb S' ∪ jf S')＊ ≡ (sb S ∪ jf S)＊ ⨾ (ES.cont_sb_dom S k × eq e ∪ jf S' ⨾ ⦗eq e⦘)^?. 
+Proof. 
+  cdes LSTEP; cdes AJF; cdes BSTEP_.
+  assert (ESBasicStep.t e e' S S') as BSTEP.
+  { econstructor. eauto. }
+  erewrite ESBasicStep.basic_step_nupd_sb. 
+  2 : { desf; eauto. }
+  rewrite <- EVENT.
+  rewrite JF'.
+  arewrite 
+    ( sb S ∪ ES.cont_sb_dom S k × eq e ∪ (jf S ∪ singl_rel w e) ≡
+     (ES.cont_sb_dom S k × eq e ∪ singl_rel w e) ∪ (sb S ∪ jf S))
+    by basic_solver. 
+  erewrite clos_refl_trans_union_ext with (r' := sb S ∪ jf S).
+  { arewrite 
+      ((jf S ∪ singl_rel w e) ⨾ ⦗eq e⦘ ≡ singl_rel w e).
+    { rewrite seq_union_l. 
+      arewrite (jf S ⨾ ⦗eq e⦘ ≡ ∅₂). 
+      { rewrite wfE.(ES.jfE).
+        unfolder; splits; ins; desf; omega. }
+      basic_solver. }
+    basic_solver. }
+  all : split; [|basic_solver].
+  all : erewrite ES.cont_sb_domE; eauto. 
+  all : arewrite (singl_rel w e ⊆ E S × eq e); [basic_solver|].
+  all : relsf.
+  2 : rewrite wfE.(ES.sbE); rewrite wfE.(ES.jfE).
+  all : unfolder; splits; ins; desf; omega.
+Qed.
+
+Lemma load_step_rf e e' S S'
+      (BSTEP : ESBasicStep.t e e' S S')
+      (LSTEP: t_load e e' S S') 
+      (wfE: ES.Wf S) : 
+  rf S' ≡ rf S ∪ (ew S)^? ⨾ jf S' ⨾ ⦗eq e⦘ \ cf S'.
+Proof.
+  cdes LSTEP; cdes AJF; cdes BSTEP; cdes BSTEP_.
+  unfold "rf" at 1.
+  rewrite EW', JF'.
+  autorewrite with hahn hahn_full.
+  rewrite minus_union_l.
+  arewrite ((ew S)^? ⨾ jf S \ cf S' ≡ rf S).
+  { unfold "rf".
+    admit. }
+  arewrite ((ew S)^? ⨾ jf S ⨾ ⦗eq e⦘ ≡ ∅₂).
+  { rewrite ES.jfE; auto.
+    rewrite !seqA.
+    split; [|done]. ESBasicStep.step_solver. }
+  arewrite (singl_rel w e ⨾ ⦗eq e⦘ ≡ singl_rel w e); 
+    basic_solver 10.
+Admitted.
+
+Lemma load_step_rf_dom e e' S S'
+      (BSTEP : ESBasicStep.t e e' S S')
+      (LSTEP: t_load e e' S S') 
+      (wfE: ES.Wf S) : 
+  dom_rel (rf S') ⊆₁ E S.
+Proof. 
+  erewrite load_step_rf; eauto. 
+  rewrite dom_union.
+  unionL.
+  { rewrite ES.rfE; auto. basic_solver. }
+  rewrite ES.ewE; auto. 
+  rewrite dom_rel_helper with (r := jf S').
+  2 : eapply load_step_jf_dom; eauto. 
+  basic_solver.
+Qed.
+
+Lemma load_step_rf_rmw e e' S S'
+      (BSTEP : ESBasicStep.t e e' S S')
+      (LSTEP: t_load e e' S S') 
+      (wfE: ES.Wf S) : 
+  rf S' ⨾ rmw S' ≡ rf S ⨾ rmw S.
+Proof. 
+  cdes LSTEP; cdes AJF; cdes BSTEP; cdes BSTEP_.
+  rewrite ESBasicStep.basic_step_nupd_rmw; eauto.
+  unfold "rf". 
+  rewrite JF', EW'.
+  rewrite seq_union_r, minus_union_l, seq_union_l.
+  arewrite (((ew S)^? ⨾ singl_rel w e \ cf S') ⨾ rmw S ≡ ∅₂). 
+  { rewrite crE. 
+    rewrite seq_union_l. 
+    rewrite minus_union_l.
+    rewrite seq_union_l. 
+    rewrite seq_id_l.
+    unfold same_relation; splits; [|basic_solver].
+    rewrite ES.rmwE; auto.
+    apply inclusion_union_l;
+      unfolder; ins; splits; desf; omega. }
+  rewrite union_false_r.
+  admit.
+Admitted.
+
+Lemma load_step_cc lang k k' st st' e e' S S'
+      (BSTEP_ : ESBasicStep.t_ lang k k' st st' e e' S S') 
+      (LSTEP: t_load e e' S S') 
+      (wfE: ES.Wf S) :
+  cc S' ≡ cc S ∪ 
+     ES.cont_cf_dom S k × eq e ∩ 
+     (jfe S ⨾ (sb S ∪ jf S)＊ ⨾ (jfe S ⨾ ES.cont_sb_dom S k × eq e ∪ jfe S')). 
+Proof. 
+  cdes LSTEP; cdes AJF; cdes BSTEP_.
+  assert (ESBasicStep.t e e' S S') as BSTEP.
+  { econstructor. eauto. }
+  unfold cc. 
+  erewrite load_step_sb_jf; eauto. 
+  erewrite ESBasicStep.basic_step_nupd_sb with (S' := S'). 
+  2 : { desf; eauto. }
+  erewrite ESBasicStep.basic_step_nupd_cf; eauto. 
+  2 : { desf; eauto. }
+  rewrite <- EVENT.
+  rewrite <- seqA with (r2 := jfe S').
+  arewrite
+    (((sb S ∪ jf S)＊ ⨾ (ES.cont_sb_dom S k × eq e ∪ jf S' ⨾ ⦗eq e⦘)^?) ⨾ jfe S' ≡
+     (sb S ∪ jf S)＊ ⨾ jfe S'). 
+  { rewrite seqA, crE, !seq_union_l, !seq_union_r, seq_id_l.
+    arewrite (ES.cont_sb_dom S k × eq e ⨾ jfe S' ≡ ∅₂). 
+    { apply seq_codom_dom_inter.
+      split; [|basic_solver].
+      erewrite load_step_jfe_dom; eauto. 
+      unfolder; splits; ins; desf; omega. }
+    arewrite (⦗eq e⦘ ⨾ jfe S' ≡ ∅₂).
+    { apply seq_codom_dom_inter.
+      split; [|basic_solver].
+      erewrite load_step_jfe_dom; eauto. 
+      unfolder; splits; ins; desf; omega. }
+    basic_solver 10. }
+  arewrite (jfe S' ⨾ (sb S ∪ jf S)＊ ⨾ jfe S' ≡ jfe S ⨾ (sb S ∪ jf S)＊ ⨾ jfe S').
+  { rewrite <- cr_of_ct, crE, seq_union_l, seq_union_r, seq_id_l.
+    arewrite (jfe S' ⨾ jfe S' ≡ ∅₂).
+    { erewrite load_step_jfe; eauto. 
+      relsf. split; [|basic_solver].
+      repeat apply inclusion_union_l.
+      { rewrite wfE.(ES.jfeD).
+        type_solver. }
+      { rewrite wfE.(ES.jfeE).
+        unfolder; splits; ins; desf; omega. }
+      { unfold ES.jfe. 
+        rewrite JF', <- seq_eqv_minus_lr. 
+        rewrite wfE.(ES.jfE), wfE.(ES.jfD).
+        assert (is_w (lab S) w) as WW'. 
+        { eapply ESBasicStep.type_step_eq_dom with (S' := S'); eauto. done. }
+        unfolder; splits; ins; desf; [omega | type_solver]. } 
+      rewrite seqA. 
+      rewrite <- seqA with (r2 := jfe S').
+      arewrite (⦗eq e⦘ ⨾ jfe S' ⊆ ∅₂); [|basic_solver].
+      apply seq_codom_dom_inter.
+      split; [|basic_solver].
+      erewrite load_step_jfe_dom; eauto. 
+      unfolder; splits; ins; desf; omega. }
+    rewrite union_false_l.
+    rewrite seq_union_r. 
+    arewrite (jfe S ⨾ jfe S' ≡ ∅₂).
+    { erewrite load_step_jfe with (S' := S'); eauto. 
+      relsf. split; [|basic_solver].
+      repeat apply inclusion_union_l.
+      { rewrite wfE.(ES.jfeD).
+        type_solver. }
+      unfold ES.jfe. 
+      rewrite JF', <- seq_eqv_minus_lr. 
+      rewrite wfE.(ES.jfE), wfE.(ES.jfD).
+      assert (is_w (lab S) w) as WW'. 
+      { eapply ESBasicStep.type_step_eq_dom with (S' := S'); eauto. done. }
+      unfolder; splits; ins; desf; [omega | type_solver]. }  
+    rewrite union_false_l, <- !seqA. 
+    apply seq_more; auto. 
+    erewrite load_step_jfe with (S' := S'); eauto. 
+    rewrite seq_union_l. 
+    arewrite ((jfe S' ⨾ ⦗eq e⦘) ⨾ tc (sb S ∪ jf S) ≡ ∅₂). 
+    { split; [|basic_solver].
+      rewrite wfE.(ES.sbE), wfE.(ES.jfE), <- !restr_relE, <- restr_union.
+      rewrite restr_ct.
+      unfolder; splits; ins; desf; omega. }
+    basic_solver. }
+  rewrite crE, !seq_union_r, seq_id_r.
+  rewrite inter_union_l. 
+  apply union_more.
+  { rewrite !inter_union_r. 
+    arewrite 
+      (cf S ∩ (jfe S ⨾ (sb S ∪ jf S)＊ ⨾ jfe S' ⨾ ES.cont_sb_dom S k × eq e) ≡ ∅₂). 
+    { split; [|basic_solver].
+      rewrite ES.cfE.
+      unfolder; splits; ins; desf; omega. }
+     arewrite (jfe S' ⨾ sb S ≡ jfe S ⨾ sb S).
+    { erewrite load_step_jfe with (S' := S'); eauto. 
+      rewrite seq_union_l, seqA.
+      arewrite (jfe S' ⨾ ⦗eq e⦘ ⨾ sb S ≡ ∅₂). 
+      { split; [|basic_solver].
+        rewrite wfE.(ES.sbE).
+        unfolder; splits; ins; desf; omega. }
+      basic_solver. }
+    arewrite (cf S ∩ (jfe S ⨾ (sb S ∪ jf S)＊ ⨾ jfe S') ≡ 
+              cf S ∩ (jfe S ⨾ (sb S ∪ jf S)＊ ⨾ jfe S )). 
+    { erewrite load_step_jfe with (S' := S'); eauto. 
+      rewrite !seq_union_r, inter_union_r. 
+      arewrite (cf S ∩ (jfe S ⨾ (sb S ∪ jf S)＊ ⨾ jfe S' ⨾ ⦗eq e⦘) ≡ ∅₂).  
+      { split; [|basic_solver].
+        rewrite ES.cfE.
+        unfolder; splits; ins; desf; omega. }
+      basic_solver 42. }
+    basic_solver 42. }
+  rewrite csE, transp_cross, inter_union_l.
+  arewrite (
+      eq e × ES.cont_cf_dom S k
+         ∩ (jfe S ⨾ (sb S ∪ jf S)＊ ⨾ jfe S'
+                ∪ (jfe S ⨾ (sb S ∪ jf S)＊ ⨾ jfe S' ⨾ sb S
+                ∪ jfe S ⨾ (sb S ∪ jf S)＊ ⨾ jfe S' ⨾ ES.cont_sb_dom S k × eq e)) 
+    ≡ ∅₂).
+  { rewrite wfE.(ES.jfeE).
+    split; [|basic_solver].
+    intros x y [[EQx _] HH].   
+    assert (E S x) as Ex.  
+    { unfolder in HH. desf. }
+    eapply ESBasicStep.basic_step_acts_set_ne; eauto. desf. }
+  rewrite union_false_r, !inter_union_r.
+  arewrite (ES.cont_cf_dom S k × eq e ∩ (jfe S ⨾ (sb S ∪ jf S)＊ ⨾ jfe S' ⨾ sb S) ≡ ∅₂). 
+  { split; [|basic_solver].
+    rewrite wfE.(ES.sbE). 
+    unfolder; splits; ins; desf; omega. }
+  arewrite (jfe S' ⨾ ES.cont_sb_dom S k × eq e ≡ jfe S ⨾ ES.cont_sb_dom S k × eq e). 
+  { erewrite load_step_jfe with (S' := S'); eauto. 
+    rewrite seq_union_l. 
+    arewrite ((jfe S' ⨾ ⦗eq e⦘) ⨾ ES.cont_sb_dom S k × eq e ≡ ∅₂).
+    { split; [|basic_solver].
+      erewrite ES.cont_sb_domE; eauto. 
+      unfolder; splits; ins; desf; omega. }
+    basic_solver 10. }
+  basic_solver 16.
+Qed.    
+
+Lemma load_step_cc_seqE e e' S S' 
+      (BSTEP : ESBasicStep.t e e' S S')
+      (LSTEP: t_load e e' S S') 
+      (wfE: ES.Wf S) : 
+  cc S' ⨾ ⦗E S⦘ ≡ cc S.
+Proof. 
+  cdes LSTEP; cdes AJF; cdes BSTEP; cdes BSTEP_.
+  rewrite load_step_cc; eauto. 
+  rewrite seq_union_l. 
+  rewrite <- lib.AuxRel.seq_eqv_inter_lr.
+  arewrite (ES.cont_cf_dom S k × eq e ⨾ ⦗E S⦘ ≡ ∅₂). 
+  { split; [|basic_solver].
+    unfolder; splits; ins; desf; omega. }
+  rewrite ccE. basic_solver 10.
+Qed.
+
+Lemma load_step_vis_mon e e' S S'
+      (BSTEP : ESBasicStep.t e e' S S')
+      (LSTEP: t_load e e' S S') 
+      (wfE: ES.Wf S) : 
+  vis S ⊆₁ vis S'. 
+Proof. 
+  cdes LSTEP; cdes AJF; cdes BSTEP; cdes BSTEP_.
+  unfold vis. 
+  intros x VIS.
+  splits; desf.
+  { eapply ESBasicStep.basic_step_acts_set_mon; eauto. }
+  arewrite (eq x ⊆₁ E S ∩₁ eq x) by basic_solver.
+  unfold set_inter. rewrite <- seq_eqv.
+  rewrite <- seqA.
+  erewrite load_step_cc_seqE; eauto. 
+  rewrite EW'.
+  etransitivity; eauto.  
+  apply seq_mori; [done|]. 
+  apply clos_refl_sym_mori. 
+  eapply ESBasicStep.basic_step_sb_mon; eauto.  
+Qed.
+  
+Lemma load_step_rs e e' S S' 
+      (BSTEP : ESBasicStep.t e e' S S')
+      (LSTEP: t_load e e' S S') 
+      (wfE: ES.Wf S) :
+  rs S' ≡ rs S.
+Proof.
+  assert (e' = None) by inv LSTEP. subst.
+  cdes LSTEP; cdes AJF; cdes BSTEP; cdes BSTEP_.
+  assert (ES.Wf S') as wfE'.
+  { admit. (* eapply step_wf; unfold t_; eauto. *) }
+  rewrite !rs_alt; auto.
+  rewrite ESBasicStep.basic_step_nupd_sb, load_step_w, load_step_rf_rmw; eauto.
+  do 2 rewrite crE.
+  relsf.
+  apply union_more; auto.
+  do 2 rewrite <- seqA.
+  rewrite (seqA ⦗E S ∩₁ W S⦘).
+  rewrite <- restr_relE.
+  rewrite restr_inter.
+  rewrite restr_union.
+  arewrite (restr_rel (E S ∩₁ W S) (ES.cont_sb_dom S k × eq e) ≡ ∅₂).
+  { rewrite restr_relE.
+    rewrite seq_eqv_cross.
+    arewrite (E S ∩₁ W S ∩₁ eq e ≡₁ ∅); [|by rewrite cross_false_r].
+    unfolder; unfold set_subset; splits; ins; desf; omega. }
+  arewrite (restr_rel (E S ∩₁ W S) (same_loc S') ≡ restr_rel (E S ∩₁ W S) (same_loc S)).
+  2: basic_solver 21.
+  do 2 rewrite <- restr_restr.
+  apply restr_rel_more; auto.
+  rewrite <- ESBasicStep.basic_step_same_loc_restr; eauto.
+Admitted.
+
+Lemma load_step_release e e' S S' 
+      (BSTEP : ESBasicStep.t e e' S S')
+      (LSTEP: t_load e e' S S') 
+      (wfE: ES.Wf S) :
+  release S' ≡ release S. 
+Proof. 
+  assert (e' = None) by inv LSTEP. subst.
+  cdes LSTEP; cdes AJF; cdes BSTEP; cdes BSTEP_.  
+  assert (ES.Wf S') as wfE'.
+  { admit. (* eapply step_wf; unfold t_; eauto. *) }
+  rewrite !release_alt; auto.
+  rewrite ESBasicStep.basic_step_nupd_sb, load_step_rel, load_step_f, load_step_rs; eauto.
+  do 2 rewrite crE.
+  relsf.
+  apply union_more; auto.
+  rewrite !seqA.
+  arewrite (ES.cont_sb_dom S k × eq e ⨾ rs S ≡ ∅₂); 
+    [|basic_solver 10].
+  rewrite rsE; auto.
+  arewrite (ES.cont_sb_dom S k × eq e ⨾ ⦗E S⦘ ≡ ∅₂); 
+    [ split; [|done]; ESBasicStep.step_solver | basic_solver ].
+Admitted.
+
+Lemma load_step_sw e e' S S' 
+      (BSTEP : ESBasicStep.t e e' S S')
+      (LSTEP: t_load e e' S S') 
+      (wfE: ES.Wf S) :
+  sw S' ≡ sw S ∪ release S ⨾ rf S' ⨾ ⦗Acq S'⦘ ⨾ ⦗eq e⦘. 
+Proof.
+  assert (e' = None) by inv LSTEP. subst.
+  cdes LSTEP; cdes AJF; cdes BSTEP; cdes BSTEP_.  
+  assert (ES.Wf S') as wfE'.
+  { admit. (* eapply step_wf; unfold t_; eauto. *) }
+  rewrite !sw_alt; auto.
+  rewrite 
+    load_step_release, load_step_rf, load_step_f, load_step_acq,
+    ESBasicStep.basic_step_nupd_sb;
+    eauto.
+  rewrite id_union.
+  rewrite !crE.
+  relsf.
+  rewrite !unionA.
+  apply union_more; auto.
+  apply union_more; auto.
+  arewrite (ES.cont_sb_dom S k × eq e ⨾ ⦗E S ∩₁ F S⦘ ≡ ∅₂) 
+    by split; [|done]; ESBasicStep.step_solver.
+  arewrite (⦗E S ∩₁ F S⦘ ⨾ ⦗eq e ∩₁ Acq S'⦘ ≡ ∅₂) 
+    by split; [|done]; ESBasicStep.step_solver.
+  rewrite <- (seqA ((jf S' ⨾ ⦗eq e⦘ ∪ ew S ⨾ jf S' ⨾ ⦗eq e⦘) \ cf S')).
+  arewrite 
+    (((jf S' ⨾ ⦗eq e⦘ ∪ ew S ⨾ jf S' ⨾ ⦗eq e⦘) \ cf S') ⨾ sb S ≡ ∅₂) 
+    by split; [|done]; ESBasicStep.step_solver.
+  relsf.
+  rewrite id_union, seq_union_r.
+  arewrite 
+    (((jf S' ⨾ ⦗eq e⦘ ∪ ew S ⨾ jf S' ⨾ ⦗eq e⦘) \ cf S') ⨾ ⦗E S ∩₁ F S ∩₁ Acq S⦘ ≡ ∅₂) 
+    by split; [|done]; ESBasicStep.step_solver.
+  arewrite 
+    (((jf S' ⨾ ⦗eq e⦘ ∪ ew S ⨾ jf S' ⨾ ⦗eq e⦘) \ cf S') ⨾ ⦗E S ∩₁ R S ∩₁ Acq S⦘ ≡ ∅₂) 
+    by split; [|done]; ESBasicStep.step_solver.
+  basic_solver 42.
+Admitted.
+
+Lemma load_step_hb lang k k' st st' e e' S S' 
+      (BSTEP_ : ESBasicStep.t_ lang k k' st st' e e' S S') 
+      (LSTEP: t_load e e' S S') 
+      (wfE: ES.Wf S) :
+  hb S' ≡ hb S ∪ 
+     (hb S)^? ⨾ (ES.cont_sb_dom S k × eq e ∪ release S ⨾ rf S' ⨾ ⦗Acq S'⦘ ⨾ ⦗eq e⦘). 
+Proof.
+  assert (e' = None) by inv LSTEP. subst.
+  assert (ESBasicStep.t e None S S') as BSTEP.
+  { econstructor. eauto. }
+  cdes LSTEP; cdes AJF; cdes BSTEP_; desf.
+  unfold hb at 1.
+  rewrite ESBasicStep.basic_step_nupd_sb, load_step_sw; eauto.
+  rewrite unionA.
+  rewrite (unionAC (ES.cont_sb_dom S k × eq (ES.next_act S))).
+  rewrite <- (unionA (sb S)).
+  rewrite unionC.
+  erewrite clos_trans_union_ext.
+  { rewrite <- cr_of_ct.
+    fold (hb S).
+    basic_solver. }
+  all : split; [|done].
+  all : rewrite load_step_rf; eauto.
+  all : rewrite ESBasicStep.basic_step_cf; eauto.
+  all : rewrite JF'.
+  all : relsf; unionL.
+  all : by ESBasicStep.step_solver.
+Qed.
+
+Lemma load_step_hb_dom e e' S S'
+      (BSTEP : ESBasicStep.t e e' S S')
+      (LSTEP: t_load e e' S S') 
+      (wfE: ES.Wf S) : 
+  dom_rel (hb S') ⊆₁ E S.
+Proof. 
+  cdes BSTEP. cdes BSTEP_. cdes LSTEP. cdes AJF.
+  rewrite load_step_hb; eauto.
+  rewrite releaseE, hbE; auto.
+  rewrite ES.cont_sb_domE; eauto.
+  basic_solver.
+Qed.  
+
+Lemma load_step_hb_seq_E e e' S S' 
+      (BSTEP : ESBasicStep.t e e' S S')
+      (LSTEP: t_load e e' S S') 
+      (wfE: ES.Wf S) :
+  hb S' ⨾ ⦗E S⦘ ≡ hb S.
+Proof. 
+  cdes BSTEP. cdes BSTEP_. cdes LSTEP. cdes AJF.
+  rewrite load_step_hb; eauto.
+  rewrite seq_union_l, !seqA.
+  arewrite (
+      (ES.cont_sb_dom S k × eq e ∪ release S ⨾ rf S' ⨾ ⦗Acq S'⦘ ⨾ ⦗eq e⦘) ⨾ ⦗E S⦘ ≡ ∅₂
+  ). 
+ { split; [|done]. 
+   rewrite load_step_rf; eauto.
+   rewrite ESBasicStep.basic_step_cf; eauto.
+   rewrite JF'.
+   ESBasicStep.step_solver. }
+  rewrite hbE; auto.
+  basic_solver 20.
+Qed.
+
+End ESstep.
